examples/Sorter.v
@@ -1,0 +1,1615 @@
+Require Import Common Core Front ZArith Structures. 
+
+
+Section t. 
+  Variable A : Type. 
+  
+  (** Sequences of length [2^n] are defined as complete binary trees, with data on the leaves *)
+
+  Inductive tree : nat -> Type :=
+  | L : forall x : A, tree 0
+  | N : forall n (l r : tree n), tree (S n). 
+
+  (** Destructors for the [tree] data-type  *)
+
+  Definition leaf (l : tree 0) : A := match l with 
+                                        | L x => x
+                                      end. 
+  
+  Definition left {n} (l : tree (S n)) : tree n := 
+    match l with 
+      | N _ l _ => l
+    end. 
+  Definition right {n} (l : tree (S n)) : tree n := 
+    match l with 
+      | N _ _ r => r
+    end. 
+
+  (**   *)
+  Fixpoint Forall {n} (t : tree n) f :=
+    match t with 
+      | L x => f x
+      | N _ l r => (Forall l f && Forall r f)%bool
+    end.  
+End t. 
+
+
+(* Setting up implicit arguments *)
+Arguments L {A} x. Arguments N {A} n l r.
+Arguments leaf {A} l. Arguments left {A n} l. Arguments right {A n} l.
+Arguments Forall {A n} _ _.  
+
+(** Map operation on trees  *)
+Fixpoint map {A B n} (f :A -> B) : tree A n -> tree B n :=
+  match n with 
+    | 0 => fun t => let x := leaf t in L (f x)
+    | S n => fun t => N _ (map f (left t)) (map f (right t))
+  end. 
+
+Module Spec. 
+  
+  (** This modules define the specification of our sorting network: we
+  implement the underlying sorting algorithm, and prove that it sorts
+  its input sequence*)
+  
+  Section t. 
+    Variable A : Type. 
+    
+    Fixpoint reverse n (t : tree A n) :=
+      match t with 
+        | L x => L x
+        | N n l r => N n
+                      (reverse n r)
+                      (reverse n l)
+      end.
+    
+    Variable (O : order A).
+    Fixpoint min_max_swap n : forall (l r : tree A n), tree A n * tree A n :=
+      match n return tree A n -> tree A n -> tree A n * tree A n with 
+        | 0 => fun l r => let (x,y) := cmp (leaf l) (leaf r) in (L x, L y)
+        | S n => fun l r => 
+                  let (a,b) := min_max_swap _ (left l) (left r) in 
+                  let (c,d) := min_max_swap _ (right l) (right r)in 
+                  (N _ a c, N _ b d)
+      end. 
+    
+    Fixpoint merge n: tree A n -> tree A n := 
+      match n with 
+        | 0 => fun t => t
+        | S k => fun t => let (a,b) := min_max_swap _ (left t) (right t) in
+                        N _ (merge _ a) (merge _ b)
+      end. 
+    
+    Fixpoint sort n : tree A n -> tree A n :=
+      match n with 
+        | 0 => fun t => t
+        | S n => fun t => 
+                  let l := left t in 
+                  let r := right t in 
+                  merge (S n) (N _ (sort _ l) (reverse _ (sort _ r)))
+    end. 
+    
+    Fixpoint list_of_tree {n} (t : tree A n) :=
+      match t with 
+        | L x => cons x nil
+        | N _ l r => List.app (list_of_tree l) (list_of_tree r)
+      end. 
+    
+    Fixpoint tree_of_list n (l: list A) : option (tree A n * list A) := 
+      match n with 
+        | 0 => match l with 
+                | nil => None
+                | cons t q => Some (L t, q)
+            end
+        | S n => do l, tl <- tree_of_list n l;
+                do r, tl <- tree_of_list n tl;
+                Some (N _ l r, tl)
+      end. 
+  End t.
+  
+  
+  Notation "t /<= a" := (Forall  t (fun x => x <= a)) (at level 79, left associativity).
+  
+  (** [l /<=\ r] means that all elements in [l] are smaller than the elements in [r] *)
+  Notation "l /<=\ r" := (Forall  r (fun a => (Forall l (fun x => x <= a)))) (at level 50).
+
+  (** [[:: l <= r]] means that all elements in the list [l] are smaller than the elements in [r]  *)
+
+  Notation "[:: l <= r ]" := (List.Forall (fun x => List.Forall (fun y => y <= x = true) l) r) (r, l at next level).
+  
+  (** [tsorted n t] holds if the tree [t] is sorted with respect to the implicit order *)
+  Inductive tsorted {A} {O : order A} : forall n, tree A n -> Prop :=
+  | tsorted_L : forall x, tsorted 0 (L  x)
+  | tsorted_N : forall n l r, tsorted n l -> tsorted n r -> 
+                         l /<=\ r = true -> tsorted _ (N  _ l r).
+  
+  (** These labeles describe the various bitonic sequences cases *)
+  Inductive bitonic_label : Type :=
+  | O | I | OI | IO | OIO | IOI | W.
+  
+  (** Appending bitonic sequences with labels [l1] and [l2] yields a
+ sequence whose label is [compose l1 l2] *)
+
+  Definition compose l1 l2 :=
+    match l1,l2 with 
+      (* O *)
+      | O, O => O
+      (* OI *)
+      | I, I => I
+      (* OI *)
+      | O, I => OI 
+      | O, OI => OI
+      | OI, I => OI
+      (* IO *)
+      | I, O => IO
+      | I, IO => IO
+      | IO, O => IO 
+      (* OIO *)
+      | O, IO 
+      | OI, O
+      | O, OIO 
+      | OIO, O 
+      | OI, IO => OIO
+      (* IOI *)
+      | I, IOI 
+      | IOI, I 
+      | I, OI 
+      | IO, I 
+      | IO, OI => IOI
+      (* W *)
+      | _, _ => W
+    end. 
+  
+  (** [label t]  computes the label associated with the sequence [t] *)
+  Fixpoint label {n} (t : tree bool n) := 
+    match t with
+      | L x => if x then I else O
+      | N  _ l r => compose (label l) (label r) 
+    end. 
+  
+  
+  Lemma label_O_x_leq : forall n (t1: tree bool n) m (t2 : tree bool m), label t1 = O -> t1 /<=\ t2 = true. 
+  Proof. 
+    induction t1. 
+    + simpl. destruct x. discriminate. 
+      intros  m t2 _. induction t2. trivial. simpl in * . rewrite IHt2_1. rewrite IHt2_2.  reflexivity.
+    + simpl. 
+      destruct (label t1_1) eqn: H1; try discriminate;
+      destruct (label t1_2) eqn: H2; try discriminate. 
+      clear H1 H2. 
+      assert (H1 := fun m t => IHt1_1 m t eq_refl). 
+      assert (H2 := fun m t => IHt1_2 m t eq_refl). 
+      clear - H1 H2. intros m t2 _. 
+      induction t2 as [ x | m s1 IH1 s2 IH2 ]. simpl. specialize (H1 _ (L  x)); specialize (H2 _ (L  x) ). simpl in *. rewrite H1, H2; trivial. 
+      simpl.                                                                                      
+      rewrite IH1. simpl. rewrite IH2. trivial. 
+  Qed. 
+
+  Require Import Equality. 
+  Lemma label_x_I_leq : forall n (t2: tree bool n) m (t1 : tree bool m), label t2 = I -> t1 /<=\ t2 = true. 
+  Proof. 
+    
+    induction t2. 
+    - simpl. destruct x; try discriminate. 
+      intros m t1 _. induction t1. 
+      destruct x; reflexivity. 
+      simpl. rewrite IHt1_1, IHt1_2. reflexivity. 
+    - simpl. intros. 
+      
+      destruct (label t2_1) eqn: H1; try discriminate;
+      destruct (label t2_2) eqn: H2; try discriminate. clear H.  
+      rewrite Bool.andb_true_iff. intuition. 
+  Qed. 
+  Hint Resolve label_O_x_leq label_x_I_leq. 
+  
+  Lemma tree_left_le_false : forall n (t: tree bool n), 
+                               (t /<= false) = true -> 
+                               label t = O.
+  Proof.
+    induction t. 
+    destruct x; simpl; auto. discriminate. 
+    simpl. intros H.  rewrite Bool.andb_true_iff in H. destruct H.  
+    specialize (IHt1 H); specialize (IHt2 H0); 
+    intuition. 
+    repeat match goal with 
+             | H : label ?t = ?x |- _ => rewrite H; clear H
+           end; simpl; auto.  
+  Qed.   
+
+  Lemma tree_le_OI : forall n (s : tree bool n), 
+                     forall m (t : tree bool m),
+                       t /<=\ s = true -> 
+                       label s = OI \/ label s = O  -> 
+                       label t = O.
+  Proof.      
+    induction s.
+    + simpl. destruct x; intuition;  try discriminate. 
+      auto using tree_left_le_false. 
+    + simpl; intros. 
+      rewrite Bool.andb_true_iff in H. destruct H.
+      specialize (IHs1 _ _ H).         specialize (IHs2 _ _ H1). 
+      destruct H0;
+        destruct (label s1) eqn: Hs1; destruct (label s2) eqn: Hs2; simpl in H0; try discriminate. intuition. intuition. intuition. intuition. 
+      
+  Qed. 
+  
+  Lemma sorted_label_disj : forall n t, tsorted n t -> 
+                                   label t = O \/ label t = OI \/ label t = I. 
+  Proof. 
+    induction t. simpl in *. destruct x; auto. 
+    simpl. intros H; inversion H.
+    injectT. 
+    intuition;
+      try solve [repeat match goal with 
+                          | H : label ?t = ?x |- _ => rewrite H; clear H
+                        end; simpl; auto].
+    exfalso; apply tree_le_OI in H5 ;[congruence | auto].
+    exfalso; apply tree_le_OI in H5 ;[congruence | auto].
+    exfalso; apply tree_le_OI in H5 ;[congruence | auto].
+    exfalso; apply tree_le_OI in H5 ;[congruence | auto].
+  Qed. 
+
+  (** converse operation on labels *)
+  Definition label_opp l :=
+    match l with 
+      | IO => OI | OI => IO | l => l
+    end. 
+  
+  (** [label] commutes with [reverse], upto [label_opp] *)
+  Lemma label_reverse n t : label (reverse _  n t) = label_opp (label t). 
+  Proof. 
+    induction t. 
+    destruct x; reflexivity. 
+    simpl; rewrite IHt1, IHt2. destruct (label t1); destruct (label t2); reflexivity. 
+  Qed. 
+  
+  Lemma label_opp_move : forall l r, label_opp l = r <-> l = label_opp r. 
+  Proof. 
+    destruct l; destruct r; simpl in *; intuition congruence. 
+  Qed. 
+
+  Lemma sorted_down_label_disj : forall n t, tsorted n (reverse _ _ t) -> 
+                                        label t = O \/ label t = IO \/ label t = I. 
+  Proof. 
+    induction t.
+    +  simpl in *. destruct x; auto. 
+    +  simpl. intros H; inversion H. injectT.
+       intuition;
+         try solve [repeat match goal with 
+                             | H : label ?t = ?x |- _ => rewrite H; clear H
+                           end; simpl; auto]; exfalso; apply tree_le_OI in H5; 
+         repeat 
+           match goal with 
+             | H: label (reverse _ ?n ?t) = ?l |- _  => rewrite label_reverse in H; 
+                                                      rewrite label_opp_move in H;
+                                                      simpl in H
+           end; try congruence;       
+       rewrite label_reverse, ? label_opp_move; simpl; auto. 
+  Qed. 
+  
+  (** a sequence is bitonic when its label is not [W] *)
+  Definition bitonic {n} (t : tree bool n) := 
+    match label t with 
+      | W => false
+      | _ => true
+    end. 
+  
+  
+  Lemma sorted_sorted_down_bitonic n (t1 t2 : tree bool n) : 
+    tsorted n t1 -> tsorted n (reverse _ _ t2) -> 
+    bitonic (N  _ t1 t2) = true. 
+  Proof. 
+    intros H1 H2. apply sorted_label_disj in H1.
+    apply sorted_down_label_disj in H2. 
+    unfold bitonic. simpl. 
+    intuition; 
+      repeat match goal with 
+               | H : label ?t = ?l |- _ => rewrite H; clear H
+             end; reflexivity. 
+  Qed. 
+  
+  Section mms. 
+    (** Some proofs about the min_max_swap function *)  
+    
+    Lemma tree_O_inversion : forall t : tree bool 0, exists x, t = L  x. 
+      dependent destruction t. 
+      exists x. 
+      reflexivity. 
+    Qed. 
+    
+    Lemma cmp_correct : forall (x y: bool), cmp x y = (min x y, max x y). 
+    Proof. 
+      intros; reflexivity. 
+    Qed.
+    
+    Ltac init := 
+      repeat match goal with 
+               | H : tree bool 0 |- _ =>                            
+                 let foo := fresh  in 
+                 assert (foo := tree_O_inversion H); 
+                   destruct foo; subst
+               | H : bool |- _ => destruct H
+               | |- _ -> _=> intros H; try discriminate; simpl              
+             end; auto. 
+    
+    Arguments min_max_swap {A} {_} n _ _. 
+    Arguments merge {A} {_} n _.
+    
+    Lemma label_min_max_swap_O_x n (l r: tree bool n) : 
+      label l = O -> 
+      let (a,b)  := min_max_swap n l r in 
+      label a = O /\ label b = label r. 
+    Proof. 
+      induction n. 
+      - init. 
+      - simpl. 
+        intros H. 
+        dependent destruction l. simpl in H. 
+        destruct (label l1) eqn:Hl; 
+          destruct (label l2) eqn:Hr; simpl; try discriminate.        
+        repeat match goal with 
+                   H : label ?l = O |- context [min_max_swap ?n ?l ?r] =>            
+                   let Heq := fresh in 
+                   destruct (min_max_swap n l r) as [? ?] eqn:Heq ;
+                     let H' := fresh in assert (H' := IHn l r H);
+                                       rewrite Heq in H'
+                                                        
+               end; simpl; intuition;         try solve [repeat match goal with 
+                                                                  | H : label ?x = _ |- _ => rewrite H in *; clear H
+                                                                end; simpl; auto]. 
+        rewrite H5, H6. clear. dependent destruction r; reflexivity. 
+    Qed.     
+  
+    Lemma label_min_max_swap_I_x n (l r: tree bool n) : 
+      label l = I -> 
+      let (a,b)  := min_max_swap n l r in 
+      label a = label r /\ label b = I. 
+    Proof. 
+      induction n. 
+      - init.  
+      - simpl. 
+        intros H. 
+        dependent destruction l. simpl in H. 
+        destruct (label l1) eqn:Hl; 
+        destruct (label l2) eqn:Hr; simpl; try discriminate.        
+        repeat 
+          match goal with 
+              H : label ?l = I |- context [min_max_swap ?n ?l ?r] =>            
+              let Heq := fresh in 
+              destruct (min_max_swap n l r) as [? ?] eqn:Heq ;
+                let H' := fresh in assert (H' := IHn l r H);
+                                  rewrite Heq in H'
+                                                   
+          end; simpl; intuition;         try solve [repeat match goal with 
+                                                             | H : label ?x = _ |- _ => rewrite H in *; clear H
+                                                           end; simpl; auto]. 
+        rewrite H4, H1. clear. dependent destruction r; reflexivity. 
+    Qed.     
+    
+    Lemma label_min_max_swap_x_I n (l r: tree bool n) : 
+      label r = I -> 
+      let (a,b)  := min_max_swap n l r in 
+      label a = label l /\ label b = I. 
+    Proof. 
+      induction n. 
+    - init.  
+    - simpl. 
+      intros H. 
+      dependent destruction r. simpl in H. 
+      destruct (label r1) eqn:Hl; 
+        destruct (label r2) eqn:Hr; simpl; try discriminate.        
+      repeat 
+        match goal with 
+            H : label ?r = I |- context [min_max_swap ?n ?l ?r] =>            
+            let Heq := fresh in 
+            destruct (min_max_swap n l r) as [? ?] eqn:Heq ;
+              let H' := fresh in assert (H' := IHn l r H);
+                                rewrite Heq in H'
+                                                 
+        end; simpl; intuition;         try solve [repeat match goal with 
+                                                           | H : label ?x = _ |- _ => rewrite H in *; clear H
+                                                         end; simpl; auto]. 
+      rewrite H4, H1. clear. dependent destruction l; reflexivity. 
+    Qed. 
+    
+    Lemma label_min_max_swap_x_O n (l r: tree bool n) : 
+      label r = O -> 
+      let (a,b)  := min_max_swap n l r in 
+      label a = O /\ label b = label l. 
+    Proof. 
+      induction n. 
+      - init.  
+      - simpl. 
+        intros H. 
+        dependent destruction r. simpl in H. 
+        destruct (label r1) eqn:Hl; 
+          destruct (label r2) eqn:Hr; simpl; try discriminate.        
+        repeat 
+          match goal with 
+              H : label ?r = O |- context [min_max_swap ?n ?l ?r] =>            
+              let Heq := fresh in 
+              destruct (min_max_swap n l r) as [? ?] eqn:Heq ;
+                let H' := fresh in assert (H' := IHn l r H);
+                                  rewrite Heq in H'
+                                                   
+          end; simpl; intuition;         try solve [repeat match goal with 
+                                                             | H : label ?x = _ |- _ => rewrite H in *; clear H
+                                                           end; simpl; auto]. 
+        rewrite H5, H6. clear. dependent destruction l; reflexivity. 
+    Qed. 
+    
+    Lemma label_min_max_swap_OI_IO n ( l r : tree bool n) :
+      label l = OI -> label r = IO -> 
+      let (a,b) := min_max_swap n l r in 
+      (label a = O /\ label b = I) \/
+      (label a = O /\ label b = IOI) \/
+      (label a = OIO /\ label b = I).
+    Proof.  
+      revert l r.  
+      induction n.  
+      - dependent destruction l. simpl; destruct x; discriminate. 
+      - intros l r; dependent destruction l; dependent destruction r. 
+        simpl. 
+        destruct (label l1) eqn:Hl1; 
+          destruct (label l2) eqn:Hl2; simpl; try discriminate;
+          destruct (label r1) eqn:Hr1; 
+          destruct (label r2) eqn:Hr2; simpl; try discriminate;
+          intros _ _;
+          destruct (min_max_swap n l1 r1) as [a b] eqn: Hab;
+          destruct (min_max_swap n l2 r2) as [c d] eqn: Hcd; 
+          simpl;
+          repeat match goal with 
+                   | H : label ?l = I, 
+                         H1 : min_max_swap ?n ?l ?r = _ |- _ => 
+                     apply (label_min_max_swap_I_x n l r) in H;
+                       rewrite H1 in H; destruct H
+                   | H : label ?l = O, 
+                         H1 : min_max_swap ?n ?l ?r = _ |- _ => 
+                     apply (label_min_max_swap_O_x n l r) in H;
+                       rewrite H1 in H; destruct H
+                   | H : label ?r = I, 
+                         H1 : min_max_swap ?n ?l ?r = _ |- _ => 
+                     apply (label_min_max_swap_x_I n l r) in H;
+                       rewrite H1 in H; destruct H
+                   | H : label ?r = O, 
+                         H1 : min_max_swap ?n ?l ?r = _ |- _ => 
+                     apply (label_min_max_swap_x_O n l r) in H;
+                       rewrite H1 in H; destruct H
+                   | Hl : label ?l = OI, 
+                          Hr : label ?r = IO, 
+                               H1 : min_max_swap ?n ?l ?r = _ |- _ => 
+                     specialize (IHn _ _ Hl Hr);
+                       rewrite H1 in IHn; intuition
+             end; try congruence;
+          try solve [repeat match goal with 
+                              | H : label ?x = _ |- _ => rewrite H in *; clear H
+                            end; simpl; auto]. 
+    Qed. 
+          
+    
+    Lemma label_min_max_swap_IO_OI n ( l r : tree bool n) :
+      label l = IO -> label r = OI -> 
+      let (a,b) := min_max_swap n l r in 
+      (label a = O /\ label b = I) \/
+      (label a = O /\ label b = IOI) \/
+      (label a = OIO /\ label b = I).
+    Proof. 
+      revert l r.  
+      induction n.  
+      - dependent destruction l. simpl; destruct x; discriminate. 
+      - intros l r; dependent destruction l; dependent destruction r. 
+        simpl. 
+        destruct (label l1) eqn:Hl1; 
+          destruct (label l2) eqn:Hl2; simpl; try discriminate;
+          destruct (label r1) eqn:Hr1; 
+          destruct (label r2) eqn:Hr2; simpl; try discriminate;
+          intros _ _;
+          destruct (min_max_swap n l1 r1) as [a b] eqn: Hab;
+          destruct (min_max_swap n l2 r2) as [c d] eqn: Hcd; 
+          simpl;
+        repeat match goal with 
+                 | H : label ?l = I, 
+            H1 : min_max_swap ?n ?l ?r = _ |- _ => 
+                   apply (label_min_max_swap_I_x n l r) in H;
+                     rewrite H1 in H; destruct H
+                 | H : label ?l = O, 
+                       H1 : min_max_swap ?n ?l ?r = _ |- _ => 
+                   apply (label_min_max_swap_O_x n l r) in H;
+                     rewrite H1 in H; destruct H
+                 | H : label ?r = I, 
+                       H1 : min_max_swap ?n ?l ?r = _ |- _ => 
+                   apply (label_min_max_swap_x_I n l r) in H;
+                     rewrite H1 in H; destruct H
+                 | H : label ?r = O, 
+                       H1 : min_max_swap ?n ?l ?r = _ |- _ => 
+                   apply (label_min_max_swap_x_O n l r) in H;
+                     rewrite H1 in H; destruct H
+                 | Hl : label ?l = IO, 
+                        Hr : label ?r = OI, 
+                             H1 : min_max_swap ?n ?l ?r = _ |- _ => 
+                   specialize (IHn _ _ Hl Hr);
+                     rewrite H1 in IHn; intuition
+               end; try congruence;
+        try solve [repeat match goal with 
+                            | H : label ?x = _ |- _ => rewrite H in *; clear H
+                          end; simpl; auto]. 
+    Qed. 
+    
+    Lemma bitonic_min_max_swap n l r :
+      bitonic (N n  l r) = true -> 
+      let (a,b) := (min_max_swap  _ l r) in 
+      bitonic a = true /\
+      bitonic b = true /\
+      a /<=\ b = true. 
+    Proof. 
+      induction n. 
+      - unfold bitonic; simpl.
+        dependent destruction l; dependent destruction r; destruct x; destruct x0; simpl; 
+        try discriminate; compute; intuition. 
+      - unfold bitonic.  replace (label (N (S n) l r)) with (compose (label l) (label r)) by reflexivity;
+        destruct (label l) eqn:Hl; 
+          destruct (label r) eqn:Hr; try discriminate; intros H; compute in H; 
+        try 
+          (clear IHn; match goal with 
+             | H : label l = O |- _ => 
+               apply (label_min_max_swap_O_x _ _ r) in H  
+             | H : label l = I |- _ => 
+               apply (label_min_max_swap_I_x _ _ r) in H
+             | H : label r = O |- _ => 
+               apply (label_min_max_swap_x_O _ l) in H
+             | H : label r = I |- _ => 
+               apply (label_min_max_swap_x_I _ l) in H          
+           end; 
+           destruct (min_max_swap _ l r) as [a b] eqn: Hab;
+           match goal with 
+               H : _ /\ _ |- _ =>  destruct H as [Hl1 Hl2]; rewrite Hl1, Hl2
+           end; 
+           match goal with 
+             | H : label ?t = ?l |- _ => rewrite H; intuition
+           end).
+        (* interesting cases: the trees have label IO and OI *)
+        pose proof (label_min_max_swap_OI_IO _ l r Hl Hr).        
+        destruct (min_max_swap _ l r) as [a b] eqn:Hab. 
+        intuition try solve [repeat match goal with 
+                                      | H : label ?x = _ |- _ => rewrite H in *; clear H
+                                    end; simpl; auto]. 
+        pose proof (label_min_max_swap_IO_OI _ l r Hl Hr).        
+        destruct (min_max_swap _ l r) as [a b] eqn:Hab. 
+        intuition try solve [repeat match goal with 
+                                      | H : label ?x = _ |- _ => rewrite H in *; clear H
+                                    end; simpl; auto]. 
+    Qed. 
+    
+    Section misc. 
+      
+      (** Various lemmas that relate operations on sequenes, and their sortedness *)
+      Lemma tree_le_N_left n t1 t2 : forall  m (t: tree bool m), 
+                                       N n t1 t2 /<=\ t = true -> 
+                                       t1 /<=\ t = true /\ t2 /<=\ t = true. 
+      Proof. 
+        induction m. 
+        - intros; init; simpl in *; apply Bool.andb_true_iff in H; intuition. 
+        - intros. dependent destruction t.  simpl in *. 
+          rewrite ? Bool.andb_true_iff in *. 
+          destruct H as [H1 H2].  apply IHm in H1; apply IHm in H2.  
+          intuition. 
+      Qed. 
+      
+      Lemma tree_le_N_left' n t1 t2 m (t: tree bool m): 
+        t1 /<=\ t = true -> t2 /<=\ t = true ->         N n t1 t2 /<=\ t = true.
+      Proof.
+        induction m. 
+        - intros; init; simpl in *; apply Bool.andb_true_iff; intuition. 
+        - intros. dependent destruction t.  simpl in *. 
+          rewrite ? Bool.andb_true_iff in *. 
+          intuition. 
+      Qed. 
+        
+      Hint Resolve tree_le_N_left' .
+      
+      Lemma tree_le_N_right n t1 t2 m (t: tree bool m): 
+        t /<=\ N n t1 t2 = true -> 
+            t /<=\ t1 = true /\ t /<=\ t2 = true. 
+      Proof. 
+        induction m. 
+        - intros; init; simpl in *; apply Bool.andb_true_iff in H; intuition. 
+        - intros. dependent destruction t.  simpl in *. 
+          apply Bool.andb_true_iff in H; intuition;
+          apply IHm in H0; 
+          apply IHm in H1; 
+          apply Bool.andb_true_iff; intuition. 
+      Qed. 
+      
+      Lemma tree_le_N_right' n t1 t2 m (t: tree bool m): 
+            t /<=\ t1 = true -> t /<=\ t2 = true -> 
+            t /<=\ N  n t1 t2 = true.
+      Proof. 
+        induction m. 
+        - intros; init; simpl in *; apply Bool.andb_true_iff; intuition. 
+        - intros. dependent destruction t.  simpl in *. 
+          rewrite ? Bool.andb_true_iff in *. 
+          intuition. 
+      Qed. 
+      Hint Resolve tree_le_N_right' .
+      
+
+      Lemma tree_le_min_max_swap_left m (t : tree bool m) : forall n t1 t2, 
+                                                              t1 /<=\ t = true -> t2 /<=\ t = true ->
+                                                              let (a,b) := (min_max_swap n t1 t2) in 
+                                                              a /<=\ t = true /\ b /<=\ t = true. 
+      Proof. 
+        induction n; dependent destruction t1; dependent destruction t2.  
+        - destruct x; destruct x0; simpl;
+          simpl; auto. 
+        - intros. simpl. 
+          destruct (min_max_swap _ t1_1 t2_1) as [a b] eqn:Hab. 
+          destruct (min_max_swap _ t1_2 t2_2) as [c d] eqn:Hcd.
+          apply tree_le_N_left in H. 
+          apply tree_le_N_left in H0. destruct H; destruct H0. 
+          pose proof (IHn t1_1 t2_1 H H0). rewrite Hab in H3. 
+          pose proof (IHn t1_2 t2_2 H1 H2). rewrite Hcd in H4. 
+          intuition. 
+      Qed. 
+      
+      Lemma tree_le_min_max_swap_right m (t : tree bool m) : forall n t1 t2, 
+                                                               t /<=\ t1 = true -> t /<=\ t2 = true ->
+                                                               let (a,b) := (min_max_swap n t1 t2) in 
+                                                               t /<=\ a = true /\ t /<=\ b = true. 
+      Proof. 
+        induction n; dependent destruction t1; dependent destruction t2.  
+        - destruct x; destruct x0; simpl;
+          simpl; auto. 
+        - intros. simpl. 
+          destruct (min_max_swap _ t1_1 t2_1) as [a b] eqn:Hab. 
+          destruct (min_max_swap _ t1_2 t2_2) as [c d] eqn:Hcd.
+          apply tree_le_N_right in H. 
+          apply tree_le_N_right in H0. destruct H; destruct H0. 
+          pose proof (IHn t1_1 t2_1 H H0). rewrite Hab in H3. 
+          pose proof (IHn t1_2 t2_2 H1 H2). rewrite Hcd in H4. 
+          intuition. 
+      Qed. 
+      
+      Lemma merge_le_left m (t2 : tree bool m) : forall n (t1 : tree bool n), 
+                                              t1 /<=\ t2 = true -> merge _ t1 /<=\ t2 = true. 
+      Proof. 
+        induction n. 
+        - dependent destruction t1. destruct x; simpl; auto. 
+        - intros. simpl. 
+          set (l := left  t1). set (r := right t1). 
+          assert (t1 = N  _ l r). dependent destruction t1; reflexivity. 
+          rewrite H0 in H. apply tree_le_N_left in H.  destruct H. 
+          pose proof (tree_le_min_max_swap_left _ _ _ _ _ H H1). 
+          destruct (min_max_swap _ l r) as [a b] eqn:Hab. 
+          intuition. 
+      Qed. 
+      
+      Lemma merge_le_right m (t2 : tree bool m) : forall n (t1 : tree bool n), 
+                                              t2 /<=\ t1 = true -> t2 /<=\ merge  _ t1 = true. 
+      Proof. 
+        induction n. 
+        - dependent destruction t1. destruct x; simpl; auto. 
+        - intros. simpl. 
+          set (l := left t1). set (r := right t1). 
+          assert (t1 = N _ l r). dependent destruction t1; reflexivity. 
+          rewrite H0 in H. apply tree_le_N_right in H.  destruct H. 
+          pose proof (tree_le_min_max_swap_right _ _ _ _ _ H H1). 
+          destruct (min_max_swap _ l r) as [a b] eqn:Hab. 
+          intuition. 
+      Qed. 
+                                
+    End misc. 
+    
+    (** Merging a bitonic sequence yields a sorted sequence  *)
+    Lemma merge_sorted : forall n (t : tree bool n), bitonic t = true -> 
+                                                tsorted _ (merge _ t).
+    Proof. 
+      induction n. 
+      - intros. simpl. dependent destruction t.  apply tsorted_L. 
+      - dependent destruction t. simpl. 
+        intros H. 
+        apply bitonic_min_max_swap in H. 
+        destruct (min_max_swap n t1 t2) as [a b] eqn: Hab. 
+        constructor. apply IHn. intuition.  
+        intuition. 
+        apply merge_le_left. apply merge_le_right. intuition. 
+    Qed. 
+    
+    (** [sort] produces a sequence that is sorted *)
+    Lemma sort_tsorted : forall n t , tsorted _ (sort _ _  n t). 
+    Proof. 
+      induction n. 
+      - intros. simpl. dependent destruction t.  apply tsorted_L. 
+      - dependent destruction t. simpl. 
+        set (l :=  (sort bool _ n t1)). 
+        set (r :=  (sort bool _  n t2)). 
+        destruct (min_max_swap n l (reverse bool n r)) as [a b] eqn: Hab. 
+        assert (bitonic (N n l (reverse bool n r))= true). 
+        apply sorted_sorted_down_bitonic. apply IHn. 
+        Lemma reverse_idempotent : forall n (t : tree bool n), reverse _ n ( reverse _ n t) = t. 
+        Proof. 
+          induction n.
+          dependent destruction t. reflexivity. 
+          intros; simpl. dependent destruction t.  simpl.  rewrite IHn.  rewrite IHn. reflexivity. 
+        Qed. 
+        rewrite reverse_idempotent. 
+        apply IHn. 
+        apply bitonic_min_max_swap in H. 
+        rewrite Hab in H. 
+        constructor; intuition. 
+        apply merge_sorted. auto. 
+        apply merge_sorted. auto. 
+        apply merge_le_left. apply merge_le_right. intuition. 
+    Qed.
+  End mms.
+  Print Assumptions sort_tsorted. 
+
+  (** * Proof of the 0-1 principle
+
+  We prove the 0-1 principle, to extend the proof of correctness of
+  our sorting algorithm from boolean sequences to sequences of an
+  arbitrary type. In order to stick with existing presentations, we
+  proved the 0-1 principle on lists, and lift this results to our
+  notion of sequences of length [2^n] *)
+
+  (** We define what it means for a list to be sorted *)
+  Inductive sorted {A} {O : order A} : list A -> Prop :=
+  | sorted_nil : sorted nil
+  | sorted_cons : forall t q, sorted q -> List.Forall (fun x => t <= x = true) q -> sorted (t::q).
+  
+  Module zero_one_principle. 
+    Section inner. 
+      Require Import Morphisms. 
+      
+      Coercion is_true (b : bool) : Prop := b = true. 
+      
+      (** We assume that we have a parametric sorting function that
+      commutes with arbitrary monotone functions *)
+
+      Variable sort : forall A, order A -> forall n, tree A n -> tree A n.
+      Hypothesis H : forall n (t : tree bool n), tsorted n (sort _ bool_order n t).
+      
+      
+      Hypothesis Hcommute : forall {A B} {PA : order A} {PB : order B} (f : A -> B) 
+                              (Hf : monotone PA PB f), 
+                            forall n t,
+                              map f (sort A PA n t)  = sort B PB n (map f t). 
+
+      
+      
+      (** If a list is not sorted, it means that one pair of
+      consecutive elemnts is not in the right order *)
+
+      Lemma not_sorted_inversion A (R: order A) : forall l, ~ sorted l -> 
+                                                       exists l1 x y l2, 
+                                                         l = List.app l1 (x :: y :: l2)%list /\ y < x .
+      Proof.
+        induction l. 
+        - intros H1. 
+          exfalso.  apply H1. constructor. 
+        - intros.  destruct l as [ | t q]. 
+          + exfalso. apply H0. constructor;  auto. constructor. 
+          + destruct (t < a) eqn : Hlt. 
+            exists nil; exists a; exists t; exists q.  simpl.  intuition. 
+            assert (~sorted (t :: q)). 
+            {
+              clear IHl. intros Hf. apply H0. clear H0. 
+              clear - Hlt Hf. assert (H : a <= t). clear - Hlt. 
+              rewrite Bool.negb_false_iff in Hlt. auto.              
+              clear Hlt. 
+              constructor. auto. inversion Hf. subst. clear - H H3.
+              constructor. auto. 
+              induction q. auto.
+              inversion H3. subst. 
+              constructor. eapply le_transitive; eauto. eauto. 
+            }
+            specialize (IHl H1).
+            destruct IHl as [l1 [x  [y [l2 [IH1 IH2] ]]]].
+            exists (a :: l1)%list; exists x; exists y; exists l2. rewrite IH1.  intuition. 
+      Qed. 
+
+      Lemma List'Forall_imply A (P Q : A -> Prop) (HPQ:forall x, P x -> Q x) : forall l, List.Forall P l -> List.Forall Q l.
+      Proof. 
+        induction l. easy.
+        intros Hal. inversion Hal. subst. constructor; intuition.
+      Qed.
+
+          
+      Lemma List'Forall_append A (P : A -> Prop) : forall l1 l2, List.Forall P l1 -> List.Forall P l2 -> 
+                                                           List.Forall P (List.app l1 l2).
+      Proof. 
+        induction l1. 
+        easy. 
+        simpl. 
+        intros. constructor. inversion H0; auto. apply IHl1.  inversion H0; auto. auto. 
+      Qed. 
+
+      Lemma List'Forall_append_inv A (P : A -> Prop) : forall l1 l2, List.Forall P (l1 ++ l2) -> List.Forall P l1 /\ List.Forall P l2. 
+      Proof.
+        induction l1. simpl. auto. 
+        intros. simpl in *. inversion H0. subst. intuition. apply IHl1 in H4. constructor; intuition.
+        apply IHl1 in H4. intuition. 
+      Qed. 
+      
+      (** Lemmas about being sorted, and various operations  *)
+      Lemma not_sorted_app : forall l1 l2, ~ sorted l2 ->  ~ sorted (List.app l1 l2).
+      Proof. 
+        induction l1. simpl. tauto. 
+        simpl. intros l2 Hl2 Hf.  
+        inversion Hf. subst.
+        apply (IHl1 l2 Hl2 H2). 
+      Qed. 
+
+      Lemma sorted_app A (R : order A):
+        forall l1 l2, sorted l1 -> sorted l2 ->
+                 [:: l1 <= l2 ] -> 
+                 sorted (l1 ++ l2). 
+      Proof. 
+        induction l1. 
+        - easy. 
+        - intros. simpl. constructor. apply IHl1. inversion H0; auto.   eauto. 
+          eapply List'Forall_imply. 2: apply H2. 
+          clear. intros. simpl in *. 
+          revert x H. induction l1. constructor.
+          intros. constructor. inversion H. subst. inversion H3; subst. subst. auto. 
+          inversion H. subst. inversion H3. subst. auto. 
+          apply List'Forall_append.
+          inversion H0; auto. 
+          
+          eapply List'Forall_imply. 2: apply H2. 
+          intros. simpl in H3. inversion H3.  subst. auto. 
+      Qed. 
+  
+      Lemma sorted_append_inversion A (O : order A): forall (l1 l2 : list A), sorted (l1 ++ l2) -> (sorted l1 /\ sorted l2). 
+      Proof. 
+        induction l1. simpl. intuition. constructor. 
+        simpl. intros. inversion H0. subst. apply IHl1 in H3. split; intuition. 
+        constructor. auto. 
+        apply List'Forall_append_inv in H4.  intuition. 
+      Qed.
+
+      Lemma List'Forall_commute A (f : A -> A -> Prop )l1 l2 :
+        List.Forall (fun x => List.Forall (fun y => f x y) l1) l2 
+        <-> List.Forall (fun y => List.Forall (fun x => f x y) l2) l1. 
+      Proof.
+        repeat setoid_rewrite List.Forall_forall. 
+        intuition. 
+      Qed.
+
+      Lemma sorted_append_order A (O : order A) : forall l1 l2, 
+                                                    sorted (l1 ++ l2) -> 
+                                                    [:: l1 <= l2].
+      Proof. 
+        induction l1. 
+        - simpl. intros l2 _. induction l2; auto. 
+        - simpl. intros. inversion H0. subst. apply IHl1 in H3. clear - H3 H4. 
+          apply List'Forall_append_inv in H4 . destruct H4. 
+          
+          rewrite List'Forall_commute. constructor. auto. 
+          rewrite List'Forall_commute. apply H3. 
+      Qed. 
+      
+      Lemma Tree'Forall_List'Forall A (P : A -> Prop) (Q : A -> bool) 
+            (IH : forall a, Q a = true -> P a):
+        forall n (t : tree A n),
+          Forall t Q -> List.Forall P (list_of_tree A t).
+      Proof.
+        induction n. dependent destruction t. simpl. intuition. 
+        dependent destruction t. simpl. intros. apply Bool.andb_true_iff in H0. destruct H0. 
+        apply List'Forall_append. auto. auto. 
+      Qed. 
+      
+      Lemma List'Forall_Tree'Forall A (P : A -> Prop) (Q : A -> bool) 
+            (IH : forall a, P a -> Q a = true ):
+        forall n (t : tree A n),
+          List.Forall P (list_of_tree A t) -> Forall t Q.
+        induction n; dependent destruction t; simpl. inversion 1. subst. apply IH. auto. 
+        intros. apply List'Forall_append_inv in H0. intuition.  apply Bool.andb_true_iff. intuition. apply IHn. auto. apply IHn. auto. 
+      Qed. 
+      
+      Lemma tsorted_sorted_list_of_tree A (R: order A): forall n (t : tree A n ), tsorted n t <-> sorted (list_of_tree A t). 
+      Proof. 
+        induction n. 
+        - dependent destruction t.  simpl. intuition. constructor. constructor.  auto.
+          inversion H0. subst. constructor. 
+        - dependent destruction t. split; intros. 
+          inversion H0; injectT. 
+          simpl.
+          apply sorted_app. rewrite <- IHn.  auto. rewrite <- IHn. auto. 
+          clear - H6. 
+          
+          eapply Tree'Forall_List'Forall. 2: apply H6. simpl. intros. 
+          eapply Tree'Forall_List'Forall. 2: apply H. simpl. intros. auto. 
+          
+          constructor. rewrite IHn. simpl in H0. 
+          
+          apply sorted_append_inversion in H0. intuition.  
+          rewrite IHn.       apply sorted_append_inversion in H0.
+          intuition.  
+          
+          simpl in H0. 
+          
+          
+          apply sorted_append_order in H0. 
+          clear - H0. 
+          eapply List'Forall_Tree'Forall. 2: apply H0. simpl. 
+          intros. eapply List'Forall_Tree'Forall. 2: apply H. 
+          simpl.
+          auto. 
+      Qed. 
+      
+      (** We are now ready for the proof of the 0-1 principle  *)
+      Theorem zero_one_principle :
+        forall A (R : order A) n t, tsorted n (sort A R  n t) .
+      Proof.
+        Require Import Classical.
+        (** We rely on a classical proof, via a double negation elimination *)
+
+        apply NNPP. 
+        intros H1.
+        apply not_all_ex_not in H1. 
+        destruct H1 as [A H1].
+        apply not_all_ex_not in H1. 
+        destruct H1 as [R H1].
+        apply not_all_ex_not in H1. 
+        destruct H1 as [n H1].
+        apply not_all_ex_not in H1. 
+        destruct H1 as [t H1].
+    
+        (** We have to prove that the hypothesis that there exists a type [A] and a list of
+   [A] that our candidate algorithm fails to sort is absurd.       *)
+
+        rewrite tsorted_sorted_list_of_tree in H1.                 
+        
+        (** From such a list, we extract a pair of consecutive
+        elements that are not in the right order*)
+
+        apply not_sorted_inversion in H1.
+        
+        destruct H1 as [l1 [x [y [ l2 [H1 H2] ]]]].
+        
+        (** We build a monotone function [f] from [A] to [Bool]*)
+        set (f := fun (c : A) => if c < x then false else true).
+        set (b := sort A R n t) in *. 
+        
+        assert (Hf : monotone _ _ f).
+        {
+          constructor.
+          intros; subst. auto. 
+          clear - f. intros. unfold f.
+          destruct  (le x a) eqn : Ha;
+            destruct  (le x b) eqn : Hb; trivial.
+          exfalso.
+          pose proof (le_transitive _ _ _ Ha H). congruence.
+        } 
+        
+        (** [f] is monotone, thus it commutes with the sort
+        function. We go on to prove that the image of our list
+        w.r.t. to [f] is not sorted.  *)
+
+        assert (~ tsorted _ (map f b)).
+        {
+          rewrite tsorted_sorted_list_of_tree. 
+          Lemma map_commute A B (f :A -> B) n (t : tree A n) : 
+            list_of_tree _ (map f t) = List.map f (list_of_tree _ t). 
+          Proof. 
+            induction n. 
+            dependent destruction t. simpl. reflexivity. 
+            simpl. repeat rewrite IHn. dependent destruction t. simpl. rewrite List.map_app. reflexivity. 
+          Qed.
+          rewrite map_commute. 
+          rewrite H1. 
+          rewrite List.map_app. simpl. 
+          apply not_sorted_app. intros Hs. 
+          inversion Hs;  subst.
+          inversion H5; subst. 
+          clear - H6 H2 f Hf.  
+          
+          assert (Hx : f x = true ). unfold f.  rewrite le_reflexive. reflexivity. 
+          assert (Hy : f y = false). unfold f. rewrite H2. reflexivity. 
+          rewrite Hx, Hy in H6. simpl in H6. discriminate. 
+        }      
+        
+        (** We now have a list of booleans that is not sorted, which
+        contradicts our hypothesis that our candidate sorting
+        algorithm succesfully sorts lists of Booleans *)
+
+        apply H0.  unfold b. 
+        
+        rewrite (Hcommute A bool _ bool_order). apply H. 
+        apply Hf. 
+      Qed. 
+  
+    End inner. 
+  End zero_one_principle.   
+  
+  (** We shall now prove that the various functions that are used in
+  the definition of our candidate sorting algorithm commute with
+  monotone functions. *)
+  
+  Section commutation_lemmas.
+    Variable A B : Type. 
+    Variable f : A -> B. 
+    Variable (PA : order A) (PB : order B). 
+    Hypothesis H : monotone PA PB f. 
+    
+    Lemma reverse_commute : 
+      forall (n : nat) (t : tree A n),
+        reverse B n (map f t) = map f (reverse A n t).  
+    Proof. 
+      induction n; dependent destruction t. 
+      - reflexivity. 
+      - simpl. rewrite ? IHn. reflexivity. 
+    Qed. 
+    
+    Lemma min_max_swap_commute :
+      forall (n : nat) (t1 t2 : tree A n) ,
+        (let (a,b) := (min_max_swap A PA n t1 t2) in 
+         (map f a, map f b)) = min_max_swap B PB n (map f t1) (map f t2). 
+    Proof. 
+      induction n; dependent destruction t1; dependent destruction t2. 
+      simpl. 
+      
+      {
+        rewrite (min_commute PA PB), (max_commute PA PB). reflexivity. auto. auto. 
+      }
+      simpl. repeat rewrite <- IHn. 
+      repeat match goal with 
+                 |- context [min_max_swap ?A ?PA ?b ?l ?r] => destruct (min_max_swap A PA b l r)
+             end. simpl. reflexivity. 
+    Qed.
+    
+    Lemma merge_commute :
+      forall (n : nat) (t : tree A n),
+        merge B PB n (map f t) = map f (merge A PA n t). 
+    Proof. 
+      induction n; dependent destruction t. 
+      - reflexivity. 
+      - simpl. rewrite <- min_max_swap_commute. 
+        destruct (min_max_swap A PA n t1 t2). simpl. rewrite IHn. rewrite IHn. reflexivity.
+    Qed. 
+  End commutation_lemmas. 
+  
+  (** * Our sort function is correct
+   We gather all the previous intermediate lemmas to prove that our
+   parametric sorting function is correct *)
+
+  Theorem sort_correct A {O : order A} cmp n (t: tree A n) : 
+    tsorted _ (sort _ cmp n t). 
+  Proof. 
+    apply zero_one_principle.zero_one_principle. 
+    apply sort_tsorted. 
+    {  
+      clear. 
+      intros.
+      induction n; dependent destruction t. 
+      - reflexivity. 
+      - simpl. 
+        destruct ( min_max_swap A PA n (sort A PA n t1)
+                                (reverse A n (sort A PA n t2))) as [a b] eqn : Hab. 
+        simpl. 
+        destruct (min_max_swap B PB n (sort B PB n (map f t1))
+                               (reverse B n (sort B PB n (map f t2)))) as [c d] eqn : Hcd. 
+        simpl. 
+        repeat rewrite <- IHn  in Hcd. 
+        repeat rewrite reverse_commute in Hcd.       
+        rewrite <- (min_max_swap_commute _ _ f PA PB) in Hcd. rewrite Hab in Hcd.  inject Hcd. 
+        repeat erewrite <- merge_commute by eassumption.  reflexivity.
+        auto. 
+    }
+  Qed. 
+End Spec. 
+
+(** * Definition of the sorting core 
+ 
+     We mimic the definition that we used in the specification with
+     the following difference. A circuit generator takes as input a
+     sequence of variables (of length [2^n]), and produces a circuit
+     with a return type [domain n] that corresponds to a
+     deep-embedding of [tree n] in our data-type of circuits.
+
+*)
+
+Module Circuit. 
+  
+  Section t. 
+    Require Import Front.
+    
+  Variable A : type.
+  Variable Var : type -> Type. 
+
+  Notation T n := (tree (expr Var A) n). 
+  Notation "x ⊗ y" := (Ttuple [x;y]) (at level 74). 
+  
+  Fixpoint domain n := 
+    match n with 
+      | 0 => A
+      | S n => (domain n) ⊗ (domain n)
+    end. 
+    
+  Definition C n := action nil Var (domain n). 
+  
+  Fixpoint reverse n (t : T n) : C n  :=
+    match t with 
+      | L x => ret (x)
+      | N n l r => 
+        do r <- reverse n r;
+        do l <- reverse n l;
+        ret [tuple r, l]
+    end%action.
+
+  Definition leaf (l : T 0) : expr Var A := match l with
+                                     | L x => x
+                                   end.
+  
+  Definition left {n} (l : T (S n)) : T n :=
+    match l with 
+      | N _ l _ => l
+    end.
+ 
+  Definition right {n} (l : T (S n)) : T n := 
+    match l with 
+      | N _ _ r => r
+    end. 
+  
+  (** The [cmp] parameter corresponds to the primitive compare and
+  swap operation that is the basic block of our sorting network. *)
+  Variable cmp : expr Var A -> expr Var A -> action nil Var (Ttuple [A ; A]). 
+  
+  Notation mk_N x y := ([tuple x,y])%expr.
+  
+  Notation "'do' x , y <- a ; b" := 
+    (do na <- a;
+     do x <- ret (Efst na);
+     do y <- ret (Efst (Esnd na));
+     b)%action
+       (at level 200, x ident, y ident, a at level 100, b at level 200): action_scope.  
+
+  Fixpoint min_max_swap n : forall (l r : T n), C (S n) :=
+    match n return T n -> T n -> action nil Var ((domain n) ⊗ (domain n)) with 
+      | 0 => fun l r => cmp (leaf l) (leaf r)
+      | S n => fun l r => 
+                do a,b <- min_max_swap n (left l) (left r);
+                do c,d <- min_max_swap n (right l) (right r); 
+                ret ([tuple mk_N a c, mk_N b d])
+    end%action. 
+
+  (* (*  The classic bind  *) *)
+  (* Notation "'do' x <~ a ; b " := (Bind a (fun x =>  b))  *)
+  (*                               (at level 200, x ident, a at level 100, b at level 200)  *)
+  (*                                : action_scope.  *)
+
+  Fixpoint rebind {U} n : expr Var (domain n) -> (T n -> action nil Var U) -> action nil Var U :=
+    match n with 
+      | 0 => fun t f => f (L t)  
+      | S n => fun t f => 
+                do a, b <- ret t;
+                rebind n a (fun t1 =>
+                              rebind n b (fun t2 =>
+                                            f (N n t1 t2)
+                                         )
+                           )
+    end%action. 
+
+  Notation "'do' x <: a ; b" :=  
+    ( 
+     rebind _ a (fun x =>  b))%action 
+      (at level 200, x ident, a at level 100, b at level 200) 
+    : action_scope. 
+
+    
+  
+  Fixpoint merge n: T n -> C n := 
+    match n with 
+      | 0 => fun t => ret (leaf t)
+      | S k => fun t => 
+                let l := left t in
+                let r := right t in
+                do a,b  <-  min_max_swap _ l r;
+                do a <: a;      (* use an explicit reification step *)
+                do b <: b;      (* use an explicit reification step *)
+                do a <- merge _ a;
+                do b <- merge _ b;
+                ret (mk_N  a b)
+    end%action. 
+  
+  
+  Fixpoint sort n : T n -> C n :=
+    match n with 
+      | 0 => fun t => ret (leaf t)
+      | S n => fun t => 
+                let l := left t in 
+                let r := right t in 
+                do l <- sort _ l; 
+                do r <- sort _ r; do r <: r;
+                do r <- reverse _ r;                 
+                do x <- ret (mk_N l r);
+                rebind (S n) x (fun x => merge _ x)
+    end%action. 
+  End t.
+
+  Definition output  (t : type) (A : action nil eval_type t) : 
+    option (eval_type t) :=    
+    match Sem.eval_action  A DList.DList.nil (Diff.init []%list)  with
+      | Some p => Some (fst p)
+      | None => None
+    end. 
+
+    
+End Circuit.
+
+
+Section proof. 
+  (** * Proof of a particular instance of our sorter core: sorting machine words of a given size. *)
+  
+  Definition int_cmp_swap  {Var : type -> Type} n :=
+    fun (x y : expr Var (Tint n)) => 
+      (do c <- ret (x <= y)%expr;
+       do min <- ret (Emux c x y)%expr;
+       do max <- ret (Emux c y x)%expr;
+       @Return nil _ _  [tuple min, max]
+      )%action. 
+
+  
+  
+  Variable size : nat. 
+  Notation A := (Tint size).
+  Notation xchg := (int_cmp_swap size).
+  
+  (** To argue about the semantics of our circuit, we fix a choice of Var as eval_type  *)
+  Notation Var := eval_type.
+  
+  Instance word_order {n} : order (Word.T n).
+  refine (mk_order _ Word.le _ _ _).
+  apply Word.le_transitive.
+  apply Word.le_total. 
+  apply Word.le_antisym.
+  Defined. 
+  
+  (** The specification of our sorting algorithm  *)
+  Definition sort := Spec.sort (Word.T size) word_order. 
+
+  (** The actual circuit definition  *)
+  Notation csort n I := (Circuit.sort A eval_type xchg n (map (@Evar eval_type A) I)).
+  
+  (** The equivalence relation between the denotation of a [domain] and a [tree] *)
+  Inductive R : forall n, Var (Circuit.domain A n) -> tree (Word.T size) n -> Prop := 
+  | R_L : forall x, R 0 (x) (L x)
+  | R_N : forall n l1 l2 r1 r2, 
+            R n l1 l2 -> 
+            R n r1 r2 -> 
+            R (S n) (l1,(r1,tt)) (N n l2 r2).
+
+  Notation "x == y" := (R _ x y) (at level 80).
+  
+  
+  Lemma R_N_fst : forall n (e: eval_type (Circuit.domain A (S n))) a b, 
+                    e == (N n a b) -> 
+                    (@Tuple.fst type eval_type (Circuit.domain A n :: nil) _ e) == a.
+  Proof. 
+    inversion 1; injectT; easy. 
+  Qed. 
+  
+  Lemma R_N_snd : forall n (e: eval_type (Circuit.domain A (S n))) a b, 
+                    e == (N n a b) -> 
+                    Tuple.fst (@Tuple.snd type eval_type (Circuit.domain A n :: nil) _ ( e)) == b.
+  Proof. 
+    inversion 1; injectT; easy. 
+  Qed. 
+  
+  Hint Constructors R. 
+  Ltac R_resolve :=
+    match goal with 
+      | H : Var (Ttuple [Circuit.domain A ?n; Circuit.domain A ?n]) |- _ => destruct H; R_resolve
+      | H : Tuple.of_list _ _ |- _ => destruct H; R_resolve
+      | H :  ( ?x , ?y ) == _  |- _ => apply R_N_fst in H; simpl in H; R_resolve
+      | H :  ( ?x , ?y) == _  |- _ => apply R_N_snd in H; simpl in H; R_resolve
+      | |- _ => eassumption
+      | |- _ == _ => constructor; R_resolve
+      | |- _ == _ => eapply R_N_fst; R_resolve
+      | |- _ == _ => eapply R_N_snd; R_resolve
+    end.  
+        
+  Hint Extern 1 (_ == _)  => R_resolve. 
+
+  Require Import Equality. 
+  
+  Lemma diff_nil : (forall t : Diff.T []%list, t = Diff.init []%list).
+  Proof. 
+    dependent destruction t. compute.  reflexivity.
+  Qed. 
+  
+  Ltac destruct_a_match H :=
+    let  rec tac G :=
+         match G with 
+           | context [ match ?x with | _ => _ end] => tac x || destruct x eqn:H
+         end
+    in
+    match goal with 
+        |- ?G => tac G; try tauto
+    end. 
+
+  Ltac destruct_a_match' := let H := fresh in destruct_a_match H.
+  
+  Lemma output_bind t a : forall u b, Circuit.output u (do x <- a; b x)%action = 
+                                 do x <- (Circuit.output t a);
+                                 Circuit.output _ (b (Evar x)).
+  Proof.
+    induction a; intros. 
+    - reflexivity.
+    - unfold Circuit.output. simpl. unfold Sem.Dyn.Bind in *.  
+      destruct_a_match'.
+      destruct p. simpl. rewrite (diff_nil t0). simpl in *. 
+      destruct_a_match'. simpl. destruct p. simpl in *. rewrite (diff_nil t1). 
+      reflexivity. 
+    - unfold Circuit.output.  simpl. destruct (eval_expr B e); simpl;  reflexivity. 
+    - unfold Circuit.output.  simpl.
+      symmetry; destruct_a_match'.  
+      simpl. unfold Sem.Dyn.Bind. rewrite H.  destruct p0. simpl. 
+      rewrite (diff_nil t). 
+      reflexivity. 
+      simpl. unfold Sem.Dyn.Bind. rewrite H. reflexivity. 
+    - unfold Circuit.output. 
+      simpl. unfold Sem.Dyn.OrElse, Sem.Dyn.Bind. 
+      destruct_a_match'. simpl. destruct p. rewrite (diff_nil t0). simpl. reflexivity.
+      destruct_a_match'. destruct p; simpl. rewrite (diff_nil t0). reflexivity.  
+  Qed.
+
+  Lemma output_rebind n e e': 
+    e == e' ->
+    forall u b, Circuit.output u (Circuit.rebind A Var n (Evar e) (fun x => b x)) =
+           Circuit.output _ (b (map (@Evar eval_type A)e')).
+  Proof. 
+    intros H. 
+    induction H. 
+    - trivial.  
+    - intros. simpl. 
+      rewrite output_bind. simpl. 
+      rewrite output_bind. simpl. 
+      rewrite output_bind. simpl. 
+      rewrite IHR1. rewrite IHR2. 
+      reflexivity. 
+  Qed. 
+
+  Lemma output_reverse  n l :       
+    match Circuit.output _ (Circuit.reverse A Var n (map Evar l)) with 
+      | None => False
+      | Some e => e == Spec.reverse _ n l
+    end.  
+  Proof. 
+    induction l. 
+    simpl; constructor. 
+    simpl in *. rewrite output_bind.
+    intro_do x2 H2. rewrite output_bind.  intro_do x1 H1. 
+    constructor; auto. 
+    auto. 
+    auto. 
+  Qed.
+
+  Lemma output_bind' t a : forall u b, Circuit.output u (do x <~ a; b x)%action = 
+                                  do x <- (Circuit.output t (ret a)%action);
+                                  Circuit.output _ (b (Evar x)).
+  Proof. 
+    intros. unfold Bind'. rewrite <- output_bind. reflexivity.  
+  Qed. 
+
+  Ltac destruct_a_let := 
+    match goal with 
+        |- context [(let (_,_) := ?a in _)] => destruct a as [? ?] eqn:? 
+    end.
+      
+  Lemma output_min_max_swap n : forall l1 l2,
+    match Circuit.output _ (Circuit.min_max_swap A Var xchg 
+                                                 n (map Evar l1) (map Evar l2)) with 
+      | None => False
+      | Some e => let (a,b) := Spec.min_max_swap _ _ n l1 l2 in e ==  N _ a b
+    end.  
+  Proof. 
+    induction n; dependent destruction l1; dependent destruction l2;simpl.
+    -  unfold min, max. unfold le, word_order. 
+       destruct (Word.le x x0) eqn:H. 
+       rewrite Word.le_is_lt_or_eq in H. rewrite H. repeat constructor. 
+       rewrite Word.le_is_lt_or_eq in H. rewrite H. repeat constructor. 
+    - repeat 
+        first 
+        [
+          rewrite output_bind ; let x := fresh in let H := fresh in intro_do x H; trivial
+        | rewrite output_bind'; let x := fresh in let H := fresh in intro_do x H; trivial
+        ];
+      repeat match goal with 
+               | H : context [Circuit.min_max_swap A Var xchg n (map Evar ?l1) (map Evar ?l2)] |- _
+                 => 
+                 let H1 := fresh in 
+                 let H2 := fresh in 
+                 assert(H1 := IHn l1 l2);
+                   simpl in H1;
+                   simpl in H; rewrite H in H1; clear H
+             end; clear IHn. 
+      repeat match goal with 
+                 H : context [?x] |- context [let (_,_) := ?x in _] => destruct x eqn:?; trivial
+             end;
+      repeat match goal with 
+          | H : context [Return _]  |- _ => compute in H; inject H
+        end. 
+      R_resolve. 
+      trivial. 
+      compute in H4. discriminate. 
+      compute in H2; discriminate. 
+      trivial.
+  Qed.
+  
+  Lemma output_merge n l:         
+    match Circuit.output _ (Circuit.merge A Var xchg n (map Evar l)) with 
+      | None => False
+      | Some e => e == Spec.merge _ _ _ (l)
+    end.  
+  Proof. 
+    revert l. 
+    induction n. 
+    - dependent destruction l; constructor.  
+    - dependent destruction l. 
+      simpl. 
+      repeat 
+        (first 
+        [
+          rewrite output_bind ; let x := fresh in let H := fresh in intro_do x H; trivial
+        | rewrite output_bind'; let x := fresh in let H := fresh in intro_do x H; trivial
+        ]);  
+        repeat match goal with 
+                 | H : context [Return _]  |- _ => compute in H; try discriminate; inject H
+               end. 
+      Focus 2. 
+      
+      Ltac use_a_match_theorem_2 thm e l1 l2 :=
+        match type of thm with 
+          | (forall x y, match @?X x y with _ => _ end) =>
+            let Y :=  eval simpl in  (X l1 l2) in
+            let H := fresh in 
+            assert (H := thm l1 l2);
+            simpl in H; simpl in e;
+            rewrite e in H
+        end.
+
+      Ltac use_a_match_theorem_1 thm e l1  :=
+        match type of thm with 
+          | (forall x , match @?X x  with _ => _ end) =>
+            let Y :=  eval simpl in  (X l1) in
+            let H := fresh in 
+            assert (H := thm l1);
+            simpl in H; simpl in e;
+            rewrite e in H
+        end.                   
+      use_a_match_theorem_2 ( output_min_max_swap n) H0 l1 l2.  
+      auto. 
+      use_a_match_theorem_2 (output_min_max_swap n) H0 l1 l2. clear H0. 
+      revert H1. destruct_a_let. intros. 
+      erewrite output_rebind by eauto. 
+      erewrite output_rebind by eauto.  
+      rewrite output_bind. intro_do x1 Hx1.  
+      rewrite output_bind. intro_do x2 Hx2.  
+      simpl in *. 
+      use_a_match_theorem_1 (IHn ) Hx1 t.  clear Hx1. 
+      use_a_match_theorem_1 (IHn ) Hx2 t0.  clear Hx2. 
+      R_resolve. 
+      use_a_match_theorem_1 (IHn ) Hx2 t0.   auto. 
+      use_a_match_theorem_1 (IHn ) Hx1 t.   auto. 
+  Qed. 
+
+      
+
+  Lemma equiv_sort n  
+        (I : tree (Var A) n) :
+    match Circuit.output _ (csort n I) with 
+      | None => False
+      | Some e => e == (sort n I)
+    end. 
+  Proof.
+    induction n.
+    - dependent destruction I. constructor.   
+    - simpl. 
+      Ltac t IHn := 
+        match goal with 
+            |- context [Circuit.output ?t (Bind' _ _ )] => rewrite output_bind
+          | |- context [Circuit.output ?t (Bind _ _ )] => rewrite output_bind' 
+          | |- context [Circuit.output ?t (csort ?n ?I)] => 
+            let H1 := fresh "H" in 
+            let H2 := fresh "H" in 
+            assert (H1 := IHn I);
+            destruct (Circuit.output _ (csort n I)) as [?|] eqn:H2; 
+              [simpl in H2; simpl; rewrite H2; simpl|tauto]
+          | |- context [Circuit.output ?t (Circuit.reverse _ _  ?n (map Evar ?I))] => 
+          let H1 := fresh "H" in 
+          let H2 := fresh "H" in 
+          assert (H1 := output_reverse n I);
+            revert H1; destruct_a_match H2; intros H1; simpl
+          | |- context [Circuit.output ?t (Circuit.merge _ _ _  ?n (map Evar ?I))] => 
+          let H1 := fresh "H" in 
+          let H2 := fresh "H" in 
+          assert (H1 := output_merge n I);
+            revert H1; destruct_a_match H2; intros H1; simpl; simpl in H2; rewrite H2; simpl
+        end. 
+      repeat (t IHn). 
+      erewrite output_rebind by eauto. 
+      repeat (t IHn).
+      repeat (simpl; t IHn).
+      simpl. 
+      erewrite output_rebind by eauto. 
+      simpl. 
+      erewrite output_rebind by eauto. 
+      simpl.
+      
+      t IHn.
+      match goal with 
+        |- context [Circuit.output ?t (Circuit.min_max_swap _ _ _ n 
+                                                           (map Evar ?l1)
+                                                           (map Evar ?l2)
+                                     )] =>
+        let H1 := fresh "H" in 
+        let H2 := fresh "H" in 
+        assert (H1 := output_min_max_swap n l1 l2);
+          revert H1; destruct_a_match H2; intros H1; simpl; simpl in H2; rewrite H2; simpl
+      end.
+      t IHn. 
+      simpl. 
+      t IHn. 
+      simpl. 
+      
+destruct (       Spec.min_max_swap (Word.T size) word_order n 
+             (sort n (left I))
+             (Spec.reverse (Word.T size) n (sort n (right I)))) as [ a b] eqn : Hab.
+      
+      rewrite output_rebind with (e' := a). 
+      rewrite output_rebind with (e' := b). 
+      rewrite output_bind.
+      simpl. 
+      t IHn. t IHn. t IHn. simpl. 
+      destruct_a_let. 
+      simpl in *. 
+      rewrite Hab in Heqp.  inject Heqp. eauto. 
+      
+      simpl in *. rewrite Hab in H5. eapply R_N_snd. R_resolve. 
+      simpl in *. rewrite Hab in H5. eapply R_N_fst. R_resolve. 
+  Qed. 
+
+  (** The final theorem states that:
+      - the output of the circuit is never None (no failure);
+      - the output of the circuit is equivalent to the output of the specification algorithm;
+      - the output of the specification algorithm is sorted with respect to the particular order we chose
+   *)
+  Theorem circuit_sort_correct n (I : tree (Var A) n) : 
+    match Circuit.output _ (csort n I) with 
+      | None => False
+      | Some out => out == (sort n I) /\ Spec.tsorted n (sort n I)
+    end. 
+  Proof. 
+    destruct_a_match H;
+    use_a_match_theorem_1 (equiv_sort n) H (I). 
+    split; auto. apply Spec.sort_correct. apply word_order. 
+    trivial. 
+  Qed. 
+    
+    
+  Print Assumptions circuit_sort_correct. 
+End proof.
+    
+                                                   
+Definition test size n := 
+  (fun V =>
+     Close V _ _ _
+           (fun x =>  Circuit.rebind _ V _ (Evar x) (fun x => Circuit.sort (Tint size) V (int_cmp_swap size) n x))).
+
+Module sanity_check. 
+  Definition c V := Circuit.sort (Tint 8) V (int_cmp_swap 8).
+  Fixpoint build n i : (tree (Word.T 8) n * Z):=
+    match n with 
+      | 0 => (L (Word.repr 8 i), (i + 1)%Z)
+      | S n => 
+        let (r,i) := build n i in 
+        let (l,i) := build n ((i*5+3) mod 255)%Z in 
+        (N _ l r, i)
+    end.
+  Definition t k := c eval_type k (map (@Evar eval_type (Tint 8)) (fst (build k 0))). 
+  Eval compute in Sem.eval_action (t 4) _ (Diff.init nil).
+End sanity_check.
+Require Compiler. 
+Definition t := (Compiler.fesiopt _ _ (test 4 4)). 
+  
