src/Structures.v
@@ -1,0 +1,76 @@
+
+(** Total order relation  *)
+Class order (A : Type) := 
+  mk_order
+    {
+      le : A -> A -> bool;
+      le_transitive : forall x y z, le x y = true -> le y z = true -> le x z = true;
+      le_total  : forall x y , le x y = true \/ le y x = true;
+      le_antisym : forall x y, le x y = true -> le y x = true -> x = y
+    }.
+
+Notation "x <= y" := (le x y).
+Notation "x < y" := (negb (le y x)).
+
+Section ops. 
+  Context {A : Type} {O : order A}.
+  
+  (* min, max operations *)
+  Definition min x y := if x <= y then x else y. 
+  Definition max x y := if x <= y then y else x. 
+
+  (* compare and swap operation *)
+  Definition cmp (x y: A) := (min x y, max x y).
+  
+  Lemma le_reflexive : forall x, x <= x = true. 
+  Proof. 
+    intros; destruct (le_total x x); auto. 
+  Qed. 
+End ops. 
+
+
+Section monotony.
+
+  (** Monotone functions preserve le *)
+
+  Context {A B : Type} (PA : order A) (PB : order B) (f : A -> B).
+  
+  Record monotone :=
+    {
+      proper_eq : forall a b, a = b -> f a = f b;
+      proper_le :> forall a b, le a b = true -> le (f a) (f b) = true
+    }.
+  
+
+  (** min and max commute with monotone functions *)
+
+  Hypothesis Hf : monotone.
+
+  Lemma min_commute : forall (x y: A), f (min x y) = min (f x) (f y). 
+  Proof. 
+    intros. 
+    unfold min. 
+    destruct (x <= y) eqn:Hxy; destruct (f x <= f y) eqn:Hfxy; trivial. 
+    apply Hf in Hxy. congruence. 
+    destruct (le_total x y). congruence. apply Hf in H. eauto using le_antisym. 
+  Qed. 
+  
+  Lemma max_commute : forall (x y: A), f (max x y) = max (f x) (f y). 
+  Proof. 
+    intros. 
+    unfold max. 
+    destruct (x <= y) eqn:Hxy; destruct (f x <= f y) eqn:Hfxy; trivial. 
+    apply Hf in Hxy. congruence. 
+    destruct (le_total x y). congruence. apply Hf in H. eauto using le_antisym. 
+  Qed. 
+
+End monotony. 
+
+(** The natural order structures on Booleans *)
+Instance bool_order : order bool. 
+Proof. 
+  refine (mk_order bool (fun x y => negb x || y)%bool _ _ _).
+  intros [|] [|] [|]; try discriminate; reflexivity. 
+  intros [|] [|]; try discriminate; auto. 
+  intros [|] [|]; try discriminate; reflexivity. 
+Defined. 
